Progress on x64 bootstrap
Stopped before remove_labels_loop. For some reason x64_enc is not being
evaluated properly (but my state could be bad).

There are a few functions in the backend that are essentially MAPs but
are not defined that way; if they were characterised as MAPs, they would
be more amenable to parallelised evaluation.

compiler/bootstrap/evaluation/x64BootstrapScript.sml
@@ -3,9 +3,89 @@ open preamble
      to_dataBootstrapTheory
      x64_configTheory
      x64_targetTheory
+     x64_targetLib
      asmLib
 
 val _ = new_theory "x64Bootstrap";
+
+(* TODO: move *)
+val ZIP_GENLIST1 = Q.store_thm("ZIP_GENLIST1",
+  `∀l f n. LENGTH l = n ⇒ ZIP (GENLIST f n,l) = GENLIST (λx. (f x, EL x l)) n`,
+  Induct \\ rw[] \\ rw[GENLIST_CONS,o_DEF]);
+
+val MAP2i_def = Define`
+  (MAP2i f [] [] = []) /\
+  (MAP2i f (h1::t1) (h2::t2) = f 0 h1 h2::MAP2i (f o SUC) t1 t2)`;
+val _ = export_rewrites["MAP2i_def"];
+
+val MAP2i_ind = theorem"MAP2i_ind";
+
+val LENGTH_MAP2i = Q.store_thm("LENGTH_MAP2i[simp]",
+  `∀f l1 l2. LENGTH l1 = LENGTH l2 ⇒ LENGTH (MAP2i f l1 l2) = LENGTH l2`,
+  ho_match_mp_tac MAP2i_ind \\ rw[]);
+
+val EL_MAP2i = Q.store_thm("EL_MAP2i",
+  `∀f l1 l2 n. n < LENGTH l1 ∧ n < LENGTH l2 ⇒
+    EL n (MAP2i f l1 l2) = f n (EL n l1) (EL n l2)`,
+  ho_match_mp_tac MAP2i_ind \\ rw[]
+  \\ Cases_on`n` \\ fs[]);
+
+val MAP3_def = Define`
+  (MAP3 f [] [] [] = []) /\
+  (MAP3 f (h1::t1) (h2::t2) (h3::t3) = f h1 h2 h3::MAP3 f t1 t2 t3)`;
+val _ = export_rewrites["MAP3_def"];
+
+val MAP3_ind = theorem"MAP3_ind";
+
+val LENGTH_MAP3 = Q.store_thm("LENGTH_MAP3[simp]",
+  `∀f l1 l2 l3. LENGTH l1 = LENGTH l3 /\ LENGTH l2 = LENGTH l3 ⇒ LENGTH (MAP3 f l1 l2 l3) = LENGTH l3`,
+  ho_match_mp_tac MAP3_ind \\ rw[]);
+
+val EL_MAP3 = Q.store_thm("EL_MAP3",
+  `∀f l1 l2 l3 n. n < LENGTH l1 ∧ n < LENGTH l2 ∧ n < LENGTH l3 ⇒
+    EL n (MAP3 f l1 l2 l3) = f (EL n l1) (EL n l2) (EL n l3)`,
+  ho_match_mp_tac MAP3_ind \\ rw[]
+  \\ Cases_on`n` \\ fs[]);
+
+fun itlist3 f L1 L2 L3 base_value =
+  let
+    fun itl ([], [], []) = base_value
+      | itl (a :: rst1, b :: rst2, c :: rst3) = f a b c (itl (rst1, rst2, rst3))
+      | itl _ = raise mk_HOL_ERR "Lib" "itlist3" "lists of different length"
+    in
+      itl (L1, L2, L3)
+    end
+
+fun zip3 ([],[],[]) = []
+  | zip3 ((h1::t1),(h2::t2),(h3::t3)) = ((h1,h2,h3)::zip3(t1,t2,t3))
+
+val (map3_tm,mk_map3,dest_map3,is_map3) = syntax_fns4 "x64Bootstrap" "MAP3"
+
+val (m3n,m3c) = CONJ_PAIR MAP3_def
+val m3c = CONV_RULE(RESORT_FORALL_CONV(sort_vars["f","h1","h2","h3","t1","t2","t3"])) m3c
+fun MAP3_CONV conv tm =
+  let
+    val (fnn,l1,l2,l3) = dest_map3 tm
+    val (els1,_) = listSyntax.dest_list l1
+    val (els2,_) = listSyntax.dest_list l2
+    val (els3,_) = listSyntax.dest_list l3
+    val nth = ISPEC fnn m3n
+    val cth = ISPEC fnn m3c
+    val cns = rator(rator(rand(snd(strip_forall(concl cth)))))
+    fun APcons t1 t2 = MK_COMB(AP_TERM cns t2,t1)
+    fun itfn e1 e2 e3 th =
+      let
+        val ts = tl(#2(strip_comb(rand(rator(concl th)))))
+        val es = [e1,e2,e3]
+        val th1 = SPECL ts (SPECL es cth)
+      in
+        TRANS th1 (APcons th (conv (list_mk_comb(fnn,es))))
+      end
+  in
+    itlist3 itfn els1 els2 els3 nth
+  end
+
+(* -- *)
 
 val _ = Globals.max_print_depth := 10;
 
@@ -74,7 +154,7 @@ val tm1 =
 
 (* about 5 minutes *)
 
-Lib.say "eval data_to_word: ";
+val () = Lib.say "eval data_to_word: ";
 val tm0 = to_livesets_thm0 |> rconc |> rand |> rand
 val thm0 = time eval tm0;
 
@@ -111,9 +191,9 @@ val word_prog = thm0 |> rconc |> listSyntax.dest_list |> #1
 
 val num_progs = length word_prog
 
+(* TODO: replace with thread pool or work queue to avoid idle cores? *)
 local
   open Thread
-
   fun chunks_of n ls =
     let
       val (ch,rst) = split_after n ls
@@ -121,10 +201,10 @@ local
       if null rst then [ch]
       else ch::(chunks_of n rst)
     end handle HOL_ERR _ => [ls]
-
 in
-  fun parMAP str_fn chunk_size eval_fn ls =
+  fun parths str_fn chunk_size eval_fn ls =
     let
+      val num_progs = length ls
       val chs = chunks_of chunk_size ls
 
       fun do_eval n [] acc = acc
@@ -150,7 +230,7 @@ in
       fun foldthis (ch,(n,refs)) =
         let
           val r = ref []
-          val _ = Thread.fork (do_chunk ch n r, [])
+          val _ = Thread.fork (do_chunk ch n r, [Thread.EnableBroadcastInterrupt true])
         in (n-chunk_size,r::refs) end
 
       val true = Mutex.trylock mutex
@@ -162,9 +242,12 @@ in
         else (ConditionVar.wait(cvar,mutex); wait())
 
       val () = wait ()
-
-      val ths = List.concat (List.map (op!) refs)
-
+    in
+      List.concat (List.map (op!) refs)
+    end
+  fun parMAP str_fn chunk_size eval_fn ls =
+    let
+      val ths = parths str_fn chunk_size eval_fn ls
       fun mk_conv() =
         let
           val next_thm = ref ths
@@ -177,6 +260,22 @@ in
     in
       mk_conv
     end
+  fun parGENLIST str_fn chunk_size eval_fn len =
+    let
+      val ls = List.tabulate (len, I)
+      val ths = parths str_fn chunk_size eval_fn ls
+      fun mk_conv() =
+        let
+          val next_thm = ref ths
+          fun el_conv _ =
+            case !next_thm of th :: rest =>
+              let val () = next_thm := rest in th end
+        in
+          listLib.GENLIST_CONV el_conv
+        end
+      in
+        mk_conv
+      end
 end
 
 val chunk_size = 400
@@ -186,12 +285,12 @@ fun eval_fn p =
   |> (RATOR_CONV(REWR_CONV word_to_word_fn_eq) THENC
       time eval)
 
-val map_conv = parMAP str_fn chunk_size eval_fn word_prog ()
+val map_conv = parMAP str_fn chunk_size eval_fn word_prog
 
 val thm1 =
   tm1
   |> (RATOR_CONV(RAND_CONV(REWR_CONV(SYM word_to_word_fn_eq))) THENC
-      RAND_CONV(REWR_CONV thm0) THENC map_conv)
+      RAND_CONV(REWR_CONV thm0) THENC map_conv())
 
 val word_prog0_def = zDefine`
   word_prog0 = ^(thm1 |> rconc)`;
@@ -224,12 +323,12 @@ fun eval_fn p =
   |> (RATOR_CONV(REWR_CONV clash_fn_eq) THENC
       time eval)
 
-val map_conv = parMAP str_fn chunk_size eval_fn word_prog0 ()
+val map_conv = parMAP str_fn chunk_size eval_fn word_prog0
 
 val thm2 =
   tm2
   |> (RATOR_CONV(RAND_CONV(REWR_CONV(SYM clash_fn_eq))) THENC
-      RAND_CONV(REWR_CONV word_prog0_def) THENC map_conv)
+      RAND_CONV(REWR_CONV word_prog0_def) THENC map_conv())
 
 val to_livesets_thm =
   to_livesets_thm1
@@ -294,12 +393,6 @@ val LENGTH_word_prog1 =
   |> (RAND_CONV(REWR_CONV word_prog1_def) THENC
       listLib.LENGTH_CONV)
 
-(* TODO: move *)
-val ZIP_GENLIST1 = Q.store_thm("ZIP_GENLIST1",
-  `∀l f n. LENGTH l = n ⇒ ZIP (GENLIST f n,l) = GENLIST (λx. (f x, EL x l)) n`,
-  Induct \\ rw[] \\ rw[GENLIST_CONS,o_DEF]);
-(* -- *)
-
 val ZIP_GENLIST_lemma =
   MATCH_MP LENGTH_ZIP
     (TRANS LENGTH_word_prog1 (SYM LENGTH_word_prog0))
@@ -307,6 +400,42 @@ val ZIP_GENLIST_lemma =
   |> C TRANS LENGTH_word_prog1
   |> MATCH_MP ZIP_GENLIST1
   |> ISPEC (lhs(concl(x64_oracle_def)))
+
+(*
+val GENLIST_EL_ZIP_lemma = Q.prove(
+  `LENGTH l1 = n ∧ LENGTH l2 = n ⇒
+   GENLIST (λx. f (y x, EL x (ZIP (l1,l2)))) n =
+   GENLIST (λx. f (y x, (EL x l1, EL x l2))) n`,
+  rw[GENLIST_FUN_EQ,EL_ZIP])
+  |> C MATCH_MP (CONJ LENGTH_word_prog1 LENGTH_word_prog0)
+*)
+
+val x64_oracle_list_def = zDefine`
+  x64_oracle_list = ^(x64_oracle_def |> rconc |> rand)`;
+
+val x64_oracle_thm = Q.prove(
+  `n < LENGTH x64_oracle_list ⇒
+   x64_oracle n = SOME (EL n x64_oracle_list)`,
+  strip_tac
+  \\ CONV_TAC(LAND_CONV(
+       RATOR_CONV(REWR_CONV x64_oracle_def THENC
+                  REWR_CONV LET_THM THENC
+                  (RAND_CONV(REWR_CONV(SYM x64_oracle_list_def))) THENC
+                  BETA_CONV)
+       THENC BETA_CONV))
+  \\ rw[]);
+
+val LENGTH_x64_oracle_list =
+  listSyntax.mk_length(lhs(concl(x64_oracle_list_def)))
+  |> (RAND_CONV(REWR_CONV x64_oracle_list_def) THENC
+      listLib.LENGTH_CONV)
+
+val GENLIST_EL_ZIP_lemma = Q.prove(
+  `LENGTH l1 = n ∧ LENGTH l2 = n ∧ LENGTH x64_oracle_list = n ⇒
+   GENLIST (λx. f (x64_oracle x, EL x (ZIP (l1,l2)))) n =
+   MAP3 (λa (b1,b2) (c1,c2,c3). f (SOME a, ((b1,b2), (c1,c2,c3)))) x64_oracle_list l1 l2`,
+  rw[LIST_EQ_REWRITE,EL_MAP3,EL_ZIP,x64_oracle_thm,UNCURRY])
+  |> C MATCH_MP (CONJ LENGTH_word_prog1 (CONJ LENGTH_word_prog0 LENGTH_x64_oracle_list))
 
 val compile_thm0 =
   compile_oracle |> SYM
@@ -329,8 +458,403 @@ val compile_thm0 =
          RATOR_CONV(RAND_CONV(
            REWR_CONV o_DEF THENC
            ABS_CONV(RAND_CONV BETA_CONV))) THENC
-         ALL_CONV (* rewrite the EL_ZIP *)) THENC
+         REWR_CONV GENLIST_EL_ZIP_lemma THENC
+         PATH_CONV"lllraraararaa" (
+           PAIRED_BETA_CONV THENC
+           PATH_CONV"llr"(
+             REWR_CONV word_allocTheory.oracle_colour_ok_def THENC
+             REWR_CONV(CONJUNCT2 option_case_def) THENC
+             BETA_CONV))) THENC
        REWR_CONV LET_THM THENC BETA_CONV THENC
        REWR_CONV LET_THM THENC BETA_CONV))
+
+val tm3 = compile_thm0 |> rconc |> rand
+
+val check_fn = tm3 |> funpow 3 rator |> rand
+
+fun str_fn n = String.concat["eval check (",Int.toString n," remain): "]
+fun eval_fn (a,b,c) =
+  list_mk_comb(check_fn,[a,b,c]) |> time eval
+
+val x64_oracle_list_els =
+  x64_oracle_list_def |> rconc |> listSyntax.dest_list |> #1
+val word_prog1_els =
+   word_prog1_def |> rconc |> listSyntax.dest_list |> #1
+val word_prog0_els =
+   word_prog0_def |> rconc |> listSyntax.dest_list |> #1
+
+val lss = zip3
+  (x64_oracle_list_els, word_prog1_els, word_prog0_els)
+
+(*
+val sum = foldr (op +) 0
+fun avg ls = sum ls div num_progs
+avg (map term_size x64_oracle_list_els)
+avg (map term_size word_prog1_els)
+avg (map term_size word_prog0_els)
+avg (map (term_size o rconc) map3els)
+*)
+
+val map3els = parths str_fn chunk_size eval_fn lss
+
+val check_fn_def = zDefine`
+  check_fn = ^check_fn`
+
+fun make_abbrevs str n [] acc = acc
+  | make_abbrevs str n (t::ts) acc =
+    let
+      val nm = str^(Int.toString n)
+      val def = new_definition(nm,mk_eq(mk_var(nm,type_of t),t))
+    in
+      make_abbrevs str (n-1) ts (def::acc)
+    end
+
+val word_prog1_defs = make_abbrevs "word_prog1_el_" num_progs word_prog1_els []
+
+fun intro_abbrev [] tm = raise UNCHANGED
+  | intro_abbrev (ab::abbs) tm =
+      FORK_CONV(REWR_CONV(SYM ab),intro_abbrev abbs) tm
+
+val word_prog1_thm =
+  word_prog1_def |> CONV_RULE(RAND_CONV(intro_abbrev (List.rev word_prog1_defs)))
+
+val map3els' =
+  mapi (fn i =>
+    CONV_RULE(
+      LAND_CONV(
+        funpow 3 RATOR_CONV(REWR_CONV(SYM check_fn_def)) THENC
+        RATOR_CONV(RAND_CONV(REWR_CONV(SYM(List.nth(word_prog1_defs,i))))))))
+  map3els
+
+local
+  val next_thm = ref map3els'
+  val remain = ref num_progs
+  fun el_conv _ =
+    case !next_thm of th :: rest =>
+      let
+        val () = next_thm := rest
+        val () = Lib.say(String.concat[Int.toString(!remain)," "])
+        val () = remain := !remain-1
+      in th end
+in
+  val map3_conv = MAP3_CONV el_conv
+end
+
+val compile_thm1 =
+  compile_thm0
+  |> CONV_RULE(RAND_CONV(
+       RAND_CONV (
+         RATOR_CONV(RATOR_CONV(RATOR_CONV(RAND_CONV(REWR_CONV(SYM check_fn_def))))) THENC
+         RAND_CONV(REWR_CONV word_prog0_def) THENC
+         RATOR_CONV(RAND_CONV(REWR_CONV word_prog1_thm)) THENC
+         RATOR_CONV(RATOR_CONV(RAND_CONV(REWR_CONV x64_oracle_list_def))) THENC
+         time map3_conv)))
+
+val word_prog2_def = zDefine`
+  word_prog2 = ^(compile_thm1 |> rconc |> rand)`;
+
+val compile_thm1' = compile_thm1
+  |> CONV_RULE(RAND_CONV(RAND_CONV(REWR_CONV(SYM word_prog2_def))))
+
+val () = computeLib.extend_compset[computeLib.Defs[word_prog2_def]] cs;
+
+(* about 15 minutes - could be parallelised? *)
+val () = Lib.say "eval word_to_stack: "
+val from_word_thm =
+  compile_thm1'
+  |> CONV_RULE(RAND_CONV(
+       REWR_CONV from_word_def THENC
+       REWR_CONV LET_THM THENC
+       RAND_CONV(time eval) THENC
+       PAIRED_BETA_CONV THENC
+       REWR_CONV LET_THM THENC
+       BETA_CONV))
+
+val stack_prog_def = zDefine`
+  stack_prog = ^(from_word_thm |> rconc |> rand)`;
+
+val from_word_thm' = from_word_thm
+  |> CONV_RULE(RAND_CONV(RAND_CONV(REWR_CONV(SYM stack_prog_def))))
+
+val () = computeLib.extend_compset[computeLib.Defs[stack_prog_def]] cs;
+
+val bare_cs = wordsLib.words_compset()
+val () =
+  computeLib.extend_compset[computeLib.Extenders[compilerComputeLib.add_compiler_compset]] bare_cs
+val bare_eval = computeLib.CBV_CONV bare_cs
+
+val stack_to_lab_thm0 =
+  from_word_thm'
+  |> CONV_RULE(RAND_CONV(
+       REWR_CONV from_stack_def THENC
+       RAND_CONV bare_eval THENC
+       REWR_CONV LET_THM THENC BETA_CONV THENC
+       RAND_CONV(RATOR_CONV(RAND_CONV eval)) THENC
+       RAND_CONV(funpow 2 RATOR_CONV(RAND_CONV bare_eval)) THENC
+       RAND_CONV(funpow 3 RATOR_CONV(RAND_CONV bare_eval)) THENC
+       RAND_CONV(funpow 4 RATOR_CONV(RAND_CONV bare_eval)) THENC
+       REWR_CONV LET_THM THENC BETA_CONV))
+
+val tm4 = stack_to_lab_thm0 |> rconc |> rand
+
+val prog_comp_tm =
+  stack_allocTheory.prog_comp_def
+  |> SPEC_ALL |> concl |> lhs |> strip_comb |> #1
+  |> inst[alpha |-> fcpSyntax.mk_int_numeric_type 64]
+
+fun str_fn n = String.concat["eval stack_alloc (",Int.toString n," remain): "]
+fun eval_fn p = mk_comb(prog_comp_tm,p) |> time eval
+
+val stack_prog_els =
+  stack_prog_def |> rconc |> listSyntax.dest_list |> #1
+
+val map_conv = parMAP str_fn chunk_size eval_fn stack_prog_els
+
+val stack_alloc_thm =
+  tm4 |>
+  (REWR_CONV stack_to_labTheory.compile_def THENC
+   RAND_CONV(
+     REWR_CONV stack_allocTheory.compile_def THENC
+     FORK_CONV(eval,
+       RAND_CONV(REWR_CONV stack_prog_def) THENC
+       map_conv()) THENC
+     listLib.APPEND_CONV))
+
+val stack_alloc_prog_def = zDefine`
+  stack_alloc_prog = ^(stack_alloc_thm |> rconc |> rand)`;
+
+val stack_to_lab_thm1 =
+  stack_to_lab_thm0
+  |> CONV_RULE(RAND_CONV(
+       RAND_CONV (
+         REWR_CONV stack_alloc_thm THENC
+         RAND_CONV(REWR_CONV(SYM stack_alloc_prog_def)) THENC
+         REWR_CONV LET_THM THENC BETA_CONV)))
+
+val tm5 = stack_to_lab_thm1 |> rconc |> rand
+
+val stack_remove_thm0 =
+  tm5 |>
+  (RAND_CONV(
+    RATOR_CONV(RAND_CONV eval) THENC
+    funpow 3 RATOR_CONV(RAND_CONV bare_eval) THENC
+    funpow 4 RATOR_CONV(RAND_CONV eval) THENC
+    REWR_CONV stack_removeTheory.compile_def THENC
+    LAND_CONV eval))
+
+val tm6 = stack_remove_thm0 |> rconc |> rand |> rand
+
+val prog_comp_n_tm = tm6 |> rator |> rand
+
+fun str_fn n = String.concat["eval stack_remove (",Int.toString n," remain): "]
+
+fun eval_fn p = mk_comb(prog_comp_n_tm,p) |> time eval
+
+val stack_alloc_prog_els =
+  stack_alloc_prog_def |> rconc |> listSyntax.dest_list |> #1
+
+val map_conv = parMAP str_fn chunk_size eval_fn stack_alloc_prog_els
+
+val stack_remove_thm =
+  stack_remove_thm0
+  |> CONV_RULE(RAND_CONV(
+     RAND_CONV(
+       RAND_CONV (
+         RAND_CONV(REWR_CONV stack_alloc_prog_def) THENC
+         map_conv()) THENC
+       listLib.APPEND_CONV)))
+
+val stack_remove_prog_def = zDefine`
+  stack_remove_prog = ^(stack_remove_thm |> rconc |> rand)`;
+
+val stack_to_lab_thm2 =
+  stack_to_lab_thm1
+  |> CONV_RULE(RAND_CONV(
+       RAND_CONV(
+         REWR_CONV stack_remove_thm THENC
+         RAND_CONV(REWR_CONV(SYM stack_remove_prog_def)) THENC
+         REWR_CONV LET_THM THENC BETA_CONV THENC
+         RAND_CONV(RATOR_CONV(RAND_CONV eval)) THENC
+         REWR_CONV LET_THM THENC BETA_CONV THENC
+         RAND_CONV(REWR_CONV stack_namesTheory.compile_def))))
+
+val tm7 = stack_to_lab_thm2 |> rconc |> rand |> rand
+
+val prog_comp_nm_tm = tm7 |> rator |> rand
+
+fun str_fn n = String.concat["eval stack_names (",Int.toString n," remain): "]
+fun eval_fn p = mk_comb(prog_comp_nm_tm,p) |> time eval
+
+val stack_remove_prog_els =
+  stack_remove_prog_def |> rconc |> listSyntax.dest_list |> #1
+
+val map_conv = parMAP str_fn chunk_size eval_fn stack_remove_prog_els
+
+val stack_names_thm0 =
+  tm7
+  |> (RAND_CONV(REWR_CONV stack_remove_prog_def) THENC
+      map_conv ())
+
+val stack_names_prog_def = zDefine`
+  stack_names_prog = ^(stack_names_thm0 |> rconc)`;
+
+val stack_names_thm = stack_names_thm0
+  |> CONV_RULE(RAND_CONV(REWR_CONV(SYM stack_names_prog_def)))
+
+val stack_to_lab_thm3 =
+  stack_to_lab_thm2
+  |> CONV_RULE(RAND_CONV(RAND_CONV(
+       RAND_CONV(REWR_CONV stack_names_thm))))
+
+val tm8 = stack_to_lab_thm3 |> rconc |> rand
+
+val prog_to_section_tm = tm8 |> rator |> rand
+
+fun str_fn n = String.concat["eval stack_to_lab (",Int.toString n," remain): "]
+fun eval_fn p = mk_comb(prog_to_section_tm,p) |> time eval
+
+val stack_names_prog_els =
+  stack_names_prog_def |> rconc |> listSyntax.dest_list |> #1
+
+val map_conv = parMAP str_fn chunk_size eval_fn stack_names_prog_els
+
+val stack_to_lab_thm =
+  stack_to_lab_thm3
+  |> CONV_RULE(RAND_CONV(RAND_CONV(
+       RAND_CONV(REWR_CONV stack_names_prog_def) THENC
+       map_conv())))
+
+val lab_prog_def = zDefine`
+  lab_prog = ^(stack_to_lab_thm |> rconc |> rand)`;
+
+val lab_to_target_thm0 =
+  stack_to_lab_thm
+  |> CONV_RULE(RAND_CONV(
+       RAND_CONV(REWR_CONV(SYM lab_prog_def)) THENC
+       REWR_CONV from_lab_def THENC
+       RATOR_CONV(RAND_CONV bare_eval)))
+
+val tm9 = lab_to_target_thm0 |> rconc
+
+(* about 2 minutes, but could have been parallelised if filter_skip were
+   written as MAP *)
+
+val filter_skip_thm =
+  tm9 |> (
+    REWR_CONV lab_to_targetTheory.compile_def THENC
+    RAND_CONV(RAND_CONV(REWR_CONV lab_prog_def) THENC time eval))
+
+val skip_prog_def = zDefine`
+  skip_prog = ^(filter_skip_thm |> rconc |> rand)`;
+
+val filter_skip_thm' = filter_skip_thm
+  |> CONV_RULE(RAND_CONV(RAND_CONV(REWR_CONV(SYM skip_prog_def))))
+
+(* similar *)
+
+val ffi_limit_thm =
+  ``find_ffi_index_limit skip_prog``
+  |> (RAND_CONV(REWR_CONV skip_prog_def) THENC time eval)
+
+val lab_to_target_thm1 =
+  lab_to_target_thm0
+  |> CONV_RULE (RAND_CONV(
+     REWR_CONV filter_skip_thm' THENC
+     REWR_CONV lab_to_targetTheory.compile_lab_def THENC
+     RAND_CONV(REWR_CONV ffi_limit_thm) THENC
+     REWR_CONV LET_THM THENC BETA_CONV))
+
+val tm10 = lab_to_target_thm1 |> rconc |> rator |> rator |> rand
+
+val () = computeLib.extend_compset[computeLib.Extenders[x64_targetLib.add_x64_encode_compset]] cs;
+
+val remove_labels_thm0 =
+  tm10 |>
+  (REWR_CONV lab_to_targetTheory.remove_labels_def THENC
+   RAND_CONV(
+     REWR_CONV lab_to_targetTheory.enc_sec_list_def THENC
+     RAND_CONV eval THENC
+     REWR_CONV LET_THM THENC BETA_CONV THENC
+     PATH_CONV"lrlr"eval) THENC
+   PATH_CONV"lllr"eval THENC
+   PATH_CONV"lr"eval)
+
+val tm11 = remove_labels_thm0 |> rconc |> rand
+
+val enc_sec_tm = tm11 |> rator |> rand
+
+val skip_prog_els = skip_prog_def |> rconc |> listSyntax.dest_list |> #1
+
+fun str_fn n = String.concat["eval enc_sec (",Int.toString n," remain): "]
+fun eval_fn p = mk_comb(enc_sec_tm,p) |> time eval
+
+(* slow, >20 mins *)
+
+val map_conv = parMAP str_fn chunk_size eval_fn skip_prog_els
+
+val remove_labels_thm1 =
+  remove_labels_thm0
+  |> CONV_RULE(RAND_CONV(
+       RAND_CONV(
+         RAND_CONV(REWR_CONV skip_prog_def) THENC
+         map_conv())))
+
+val encoded_prog_def = zDefine`
+  encoded_prog = ^(remove_labels_thm1 |> rconc |> rand)`;
+
+(*
+val alloc_fn_def = zDefine`alloc_fn ^args = ^body`
+val alloc_fn_eq =
+  alloc_fn_def
+  |> SPEC_ALL
+  |> PairRules.PABS args
+  |> CONV_RULE(LAND_CONV PairRules.PETA_CONV)
+val alloc_fn = alloc_fn_eq|>concl|>lhs
+
+val outer_alloc_fn_intro = tm3 |> rator |> rand
+  |> ABS_CONV(RATOR_CONV(REWR_CONV(SYM alloc_fn_eq)))
+
+val outer_alloc_fn = outer_alloc_fn_intro |> rconc
+
+val word_prog1 = word_prog1_def |> concl |> lhs
+
+fun str_fn n = String.concat["eval el1 (",Int.toString n," remain): "]
+
+val el_ths1 = parths str_fn chunk_size eval_fn (List.tabulate (num_progs,I))
+*)
+
+local
+  val (EL_HD,EL_SUC) = CONJ_PAIR EL_restricted
+  val sucpre = SUC_PRE |> CONV_RULE(RAND_CONV SYM_CONV) |> SYM |> Q.GEN`m`
+in
+  fun my_el_conv tm =
+    let
+      val (n,ls) = listSyntax.dest_el tm
+      val eqsuc =
+        sucpre |> SPEC n |> CONV_RULE(RAND_CONV numLib.REDUCE_CONV)
+        |> EQT_ELIM
+        |> CONV_RULE(RAND_CONV(RAND_CONV numLib.REDUCE_CONV))
+    in
+      (RATOR_CONV(RAND_CONV(REWR_CONV eqsuc)) THENC
+       REWR_CONV EL_SUC THENC
+       my_el_conv) tm
+    end handle HOL_ERR _ =>
+      (RATOR_CONV(REWR_CONV EL_HD) THENC REWR_CONV HD) tm
+end
+
+(*
+fun str_fn n = String.concat["eval alloc (",Int.toString n," remain): "]
+fun eval_fn i =
+    mk_comb(outer_alloc_fn, numSyntax.term_of_int i)
+    |> (BETA_CONV THENC
+        RAND_CONV (
+          FORK_CONV(
+            RATOR_CONV(REWR_CONV x64_oracle_def),
+            FORK_CONV(
+              RAND_CONV(REWR_CONV word_prog1_def) THENC
+              listLib.EL_CONV,
+              RAND_CONV(REWR_CONV word_prog0_def) THENC
+              listLib.EL_CONV))))
+*)
 
 val _ = export_theory();
